* Correctly parse qualified name for component classifiers and properties

src/AADL/json_frontend/json_frontend.v
@@ -48,8 +48,10 @@ Import
 
 (** Oqarina library *)
 From Oqarina Require Import
-    Kernel.all
-    core.identifiers.
+    coq_utils.utils
+    AADL.Kernel.all
+    core.identifiers
+    AADL.instance.all.
 (* end hide *)
 Require Import Coq.Strings.String.
 
@@ -236,7 +238,7 @@ Fixpoint Map_JSON_To_Property_Value (j : json) : property_value :=
 Fixpoint Map_JSON_To_Property_Association (j : list json) :=
   match j with
       | (JSON__Object o) :: t =>
-        {| P := PSQN (get_string_from_json "name" (JSON__Object o)) "";
+        {| P :=  parse_psq_name(get_string_from_json "name" (JSON__Object o)) ; (* XX *)
           PV := (Map_JSON_To_Property_Value (get_json "property_value" (JSON__Object o))) |}
         :: Map_JSON_To_Property_Association  t
       | _ => [  ]
@@ -250,7 +252,7 @@ Fixpoint Map_JSON_To_Component' (fuel : nat) (c : list json) : list component :=
     | (JSON__Object f) :: t =>
        ( Component (get_identifier (JSON__Object f))
                    (Map_JSON_To_ComponentCategory (get_json "category" (JSON__Object f)))
-                   (FQN [] (Id (get_string_from_json "classifier" (JSON__Object f))) None)  (* classifier XXX incomplete*)
+                   (parse_fq_name (get_string_from_json "classifier" (JSON__Object f)))  (* classifier *)
                    (Map_JSON_To_Feature' m (get_features (JSON__Object f))) (* features *)
                    (Map_JSON_To_Component' m (get_subcomponents (JSON__Object f))) (* subcomponents *)
                    (Map_JSON_To_Property_Association (get_properties (JSON__Object f)))(* properties *)
@@ -293,18 +295,14 @@ Definition Map_JSON_Root_To_Component (AST : option string + json) :=
 Definition Map_JSON_String_To_Component (s : string) :=
     Map_JSON_Root_To_Component (from_string s).
 
-Definition test_properties := "
-{""aadl_xml"": {""components"": {""component"": {""category"": ""system"", ""features"": {}, ""subcomponents"": {""component"": {""category"": ""device"", ""features"": {}, ""subcomponents"": {}, ""identifier"": ""subcomp_subdevice"", ""properties"": {}, ""classifier"": ""subdevice.impl""}}, ""identifier"": ""main.impl"", ""properties"": {""property"": [{""name"": ""Test_Properties::a_record_property"", ""property_value"": {""record"": {""record_field"": [{""integer"": {""value"": ""10""}, ""name"": ""an_integer_field""}, {""name"": ""a_string_field"", ""string"": {""value"": ""test string""}}, {""real_range"": {""value_low"": ""5.0"", ""value_high"": ""10.0""}, ""name"": ""a_real_range_field""}]}}}, {""name"": ""Test_Properties::an_enumeration_property"", ""property_value"": {""enumeration"": {""value"": ""enum2""}}}, {""name"": ""Test_Properties::a_classifier_property"", ""property_value"": {""classifier"": {""value"": ""subdevice""}}}, {""name"": ""Test_Properties::a_reference_property"", ""property_value"": {""reference"": {""value"": ""subcomp_subdevice""}}}, {""name"": ""Test_Properties::a_list_of_list_property"", ""property_value"": {""list"": {""list"": [{""integer"": [{""value"": ""1""}, {""value"": ""2""}]}, {""integer"": [{""value"": ""3""}, {""value"": ""4""}]}]}}}, {""name"": ""Test_Properties::a_boolean_property"", ""property_value"": {""boolean"": {""value"": ""true""}}}, {""name"": ""Test_Properties::a_string_property"", ""property_value"": {""string"": {""value"": ""test string""}}}, {""name"": ""Test_Properties::a_real_range_property"", ""property_value"": {""real_range"": {""value_low"": ""5.0"", ""value_high"": ""10.0""}}}, {""name"": ""Test_Properties::a_real_unit_property"", ""property_value"": {""real_unit"": {""unit"": ""ns"", ""value"": ""10.0""}}}, {""name"": ""Test_Properties::a_negative_real_property"", ""property_value"": {""real"": {""value"": ""-10.0""}}}, {""name"": ""Test_Properties::a_real_property"", ""property_value"": {""real"": {""value"": ""10.0""}}}, {""name"": ""Test_Properties::an_integer_range_property"", ""property_value"": {""integer_range"": {""value_low"": ""5"", ""value_high"": ""10""}}}, {""name"": ""Test_Properties::an_integer_unit_property"", ""property_value"": {""integer_unit"": {""unit"": ""ms"", ""value"": ""10""}}}, {""name"": ""Test_Properties::a_negative_integer_property"", ""property_value"": {""integer"": {""value"": ""-10""}}}, {""name"": ""Test_Properties::an_integer_property"", ""property_value"": {""integer"": {""value"": ""10""}}}]}, ""classifier"": ""main.impl""}}, ""root_system"": ""main.impl""}}
+Definition Get_Instance (c : option string + list component) :=
+match c with
+| inr c' =>
+  match c' with
+  | h :: _ =>  h
+  | _ => nil_component
+  end
+| _ => nil_component
+end.
 
-".
 
-Compute from_string test_properties.
-Compute Map_JSON_String_To_Component test_properties.
-
-
-Compute Map_JSON_String_To_Component "XXX".
-
-Definition rma_test := "
-{""aadl_xml"": {""components"": {""component"": {""category"": ""system"", ""features"": {}, ""subcomponents"": {""component"": [{""category"": ""process"", ""features"": {}, ""subcomponents"": {""component"": [{""category"": ""thread"", ""features"": {}, ""subcomponents"": {}, ""identifier"": ""Task1"", ""properties"": {""property"": [{""name"": ""Deadline"", ""property_value"": {""integer_unit"": {""unit"": ""ms"", ""value"": ""1000""}}}, {""name"": ""Compute_Execution_time"", ""property_value"": {""integer_range_unit"": {""value_low"": ""0"", ""value_high"": ""3"", ""unit_high"": ""ms"", ""unit_low"": ""ms""}}}, {""name"": ""Period"", ""property_value"": {""integer_unit"": {""unit"": ""ms"", ""value"": ""1000""}}}, {""name"": ""Priority"", ""property_value"": {""integer"": {""value"": ""1""}}}, {""name"": ""Dispatch_Protocol"", ""property_value"": {""enumeration"": {""value"": ""Periodic""}}}]}, ""classifier"": ""Task.impl_1""}, {""category"": ""thread"", ""features"": {}, ""subcomponents"": {}, ""identifier"": ""Task2"", ""properties"": {""property"": [{""name"": ""Deadline"", ""property_value"": {""integer_unit"": {""unit"": ""ms"", ""value"": ""500""}}}, {""name"": ""Compute_Execution_time"", ""property_value"": {""integer_range_unit"": {""value_low"": ""0"", ""value_high"": ""5"", ""unit_high"": ""ms"", ""unit_low"": ""ms""}}}, {""name"": ""Period"", ""property_value"": {""integer_unit"": {""unit"": ""ms"", ""value"": ""500""}}}, {""name"": ""Priority"", ""property_value"": {""integer"": {""value"": ""2""}}}, {""name"": ""Dispatch_Protocol"", ""property_value"": {""enumeration"": {""value"": ""Periodic""}}}]}, ""classifier"": ""Task.impl_2""}]}, ""identifier"": ""node_a"", ""properties"": {""property"": {""name"": ""Actual_Processor_Binding"", ""property_value"": {""list"": {""reference"": {""value"": ""cpu""}}}}}, ""classifier"": ""node_a.impl""}, {""category"": ""processor"", ""features"": {}, ""subcomponents"": {}, ""identifier"": ""cpu"", ""properties"": {""property"": [{""name"": ""Scheduling_Protocol"", ""property_value"": {""list"": {""enumeration"": {""value"": ""POSIX_1003_HIGHEST_PRIORITY_FIRST_PROTOCOL""}}}}, {""name"": ""Processor_properties::Max_Prio_First"", ""property_value"": {""enumeration"": {""value"": ""high""}}}, {""name"": ""Scheduling_Protocol"", ""property_value"": {""list"": {""enumeration"": {""value"": ""POSIX_1003_HIGHEST_PRIORITY_FIRST_PROTOCOL""}}}}, {""name"": ""Deployment::Execution_Platform"", ""property_value"": {""enumeration"": {""value"": ""Native""}}}]}, ""classifier"": ""cpu.impl""}]}, ""identifier"": ""rma.impl"", ""properties"": {}, ""classifier"": ""rma.impl""}}, ""root_system"": ""rma.impl""}}".
-
-Compute Map_JSON_String_To_Component rma_test.
